qtesla/code/Hacl.Impl.QTesla.Constants.fst
@@ -3,6 +3,9 @@ module Hacl.Impl.QTesla.Constants
 open Lib.IntTypes
 open Hacl.SHA3
 
+//NS:
+//size is in terms of uint, which is abstract
+//normalize on constants is redundant
 let shake128_rate = size (normalize_term 168)
 let shake256_rate = size (normalize_term 136)
 
